README.md
@@ -11,6 +11,46 @@ The basic components are:
 I'm basically doing something like test-driven coding in Coq, where the
 `Example` environment is used for tests.
 
+## Status
+
+**tl;dr: the results in Wiedijk's paper is correct.** (That was
+exciting, wasn't it?)
+
+It turns out that Wiedijk's model is more or less correct. There's some
+subtlety in the second typing rule, which is a contraction of a couple
+rules in the version presented here (substitution and assumption). We
+can derive the contentious rule as a theorem in our model, so it's fine.
+
+There are some tedious theorems left to be proven, which are true but
+whose proof is...long and uninteresting. So if you believe them, then
+the model is correct.
+
+I may or may not finish them, they won't be terribly insightful.
+
+## Future directions
+
+It may be interesting to add structure types, or prove completeness.
+
+- It is easy to state completeness, but I expect it unpleant to prove:
+
+  ```coq
+  Theorem completeness : forall Γ Δ J,
+      well_typed (Γ ;; Δ |- CorrectContext) ->
+      proves (translate (Γ ;; Δ |- J)) ->
+      well_typed (Γ ;; Δ |- J).
+  ```
+
+  The trick would be to assemble a library of theorems about well-typed
+  judgements, analogous to the library of theorems concerning natural
+  deduction in `Logic.v`.
+- If you want to actually **use** this library, you would need to
+  develop useful results in the `SoftType.v` file concerning
+  `well_typed` judgements.
+- Structure types in Mizar can be thought of either as a finite set of
+  key-value pairs, or as a finite partial map. (From the set theoretic
+  perspective, they're equivalent.) You'd need to sketch out some typing
+  rule for them.
+
 # License
 
 Everything is under the MIT License.
@@ -25,7 +65,7 @@ Everything is under the MIT License.
 ## First-order logic encodings
 
 A lot of the inspiration for encoding natural deduction comes from
-Daniel Schepler's 
+Daniel Schepler's
 [coq-sequent-calculus](https://github.com/dschepler/coq-sequent-calculus).
 For locally nameless encoding and first-order logic considerations, I
 consulted (among the random books in my bookcase):
